Cleaned up typchecking

02Typed/Typechecking.thy
@@ -21,7 +21,7 @@ primrec erase :: "texpr \<Rightarrow> nexpr" where
 | "erase (TApp e\<^sub>1 e\<^sub>2) = NApp (erase e\<^sub>1) (erase e\<^sub>2)"
 
 primrec typecheck' :: "subst \<Rightarrow> var set \<Rightarrow> nexpr \<rightharpoonup> 
-    hexpr \<times> uexpr \<times> var set \<times> (uexpr \<times> uexpr) list " where
+    hexpr \<times> uexpr \<times> var set \<times> (uexpr \<times> uexpr) list" where
   "typecheck' \<Gamma> vs (NVar x) = (case \<Gamma> x of 
       Some t \<Rightarrow> Some (HVar x, t, vs, []) 
     | None \<Rightarrow> None)"
@@ -29,16 +29,16 @@ primrec typecheck' :: "subst \<Rightarrow> var set \<Rightarrow> nexpr \<rightha
 | "typecheck' \<Gamma> vs (NLam x e) = (
     let v = fresh vs
     in case typecheck' (\<Gamma>(x \<mapsto> Var v)) (insert v vs) e of
-        Some (e', t, vs', uni) \<Rightarrow> 
-          Some (HLam x (Var v) e', Ctor ''Arrow'' [Var v, t], vs', uni)
+        Some (e', t, vs', uni) \<Rightarrow> Some (HLam x (Var v) e', Ctor ''Arrow'' [Var v, t], vs', uni)
       | None \<Rightarrow> None)"
-| "typecheck' \<Gamma> vs (NApp e\<^sub>1 e\<^sub>2) = (case typecheck' \<Gamma> vs e\<^sub>1 of
-      Some (e\<^sub>1', Ctor k [t\<^sub>1, t\<^sub>2], vs', uni\<^sub>1) \<Rightarrow> (
-        if k = ''Arrow'' then case typecheck' \<Gamma> vs' e\<^sub>2 of
-            Some (e\<^sub>2', t\<^sub>3, vs'', uni\<^sub>2) \<Rightarrow> Some (HApp e\<^sub>1' e\<^sub>2', t\<^sub>2, vs'', (t\<^sub>1, t\<^sub>3) # uni\<^sub>1 @ uni\<^sub>2)
-          | None \<Rightarrow> None
-        else None)
-    | _ \<Rightarrow> None)"
+| "typecheck' \<Gamma> vs (NApp e\<^sub>1 e\<^sub>2) = (
+    let v = fresh vs
+    in case typecheck' \<Gamma> (insert v vs) e\<^sub>1 of 
+        Some (e\<^sub>1', t\<^sub>1, vs', uni\<^sub>1) \<Rightarrow> (case typecheck' \<Gamma> vs' e\<^sub>2 of
+            Some (e\<^sub>2', t\<^sub>2, vs'', uni\<^sub>2) \<Rightarrow> 
+              Some (HApp e\<^sub>1' e\<^sub>2', Var v, vs'', (t\<^sub>1, Ctor ''arrow'' [t\<^sub>2, Var v]) # uni\<^sub>1 @ uni\<^sub>2)
+          | None \<Rightarrow> None)
+      | None \<Rightarrow> None)"
 
 fun typeify :: "uexpr \<Rightarrow> ty" where
   "typeify (Var v) = TyVar v"
@@ -115,13 +115,32 @@ lemma [simp]: "valid_ty_subst \<Gamma> \<Longrightarrow> valid_ty_uexpr t \<Long
 lemma [simp]: "valid_ty_subst \<Gamma> \<Longrightarrow> valid_ty_subst \<Gamma>' \<Longrightarrow> valid_ty_subst (\<Gamma>(x := \<Gamma>' y))"
   by (auto simp add: valid_ty_subst_def ran_def)
 
+lemma [simp]: "valid_ty_uexpr (subst s e) \<Longrightarrow> valid_ty_subst s \<Longrightarrow> 
+    valid_ty_subst (extend_subst x e s)"
+  by (auto simp add: valid_ty_subst_def extend_subst_def ran_def)
+
+lemma [simp]: "valid_ty_uexpr e \<Longrightarrow> valid_ty_uexpr e' \<Longrightarrow> valid_ty_uexpr (subst [x \<mapsto> e'] e)"
+  and [simp]: "list_all valid_ty_uexpr es \<Longrightarrow> valid_ty_uexpr e' \<Longrightarrow> 
+    list_all valid_ty_uexpr (map (subst [x \<mapsto> e']) es)"
+proof (induction e and es rule: vars_varss.induct)
+  case (2 k es)
+  thus ?case 
+  proof (induction es)
+    case (Cons a es)
+    thus ?case 
+    proof (induction es)
+      case (Cons b es)
+      thus ?case by (induction es) simp_all
+    qed simp_all
+  qed simp_all
+qed simp_all
+
+lemma [simp]: "valid_ty_uexpr e \<Longrightarrow> valid_ty_uexprs ess \<Longrightarrow> valid_ty_uexprs (list_subst x e ess)"
+  by (induction ess rule: list_subst.induct) (auto simp add: valid_ty_uexprs_def)
+
 lemma [simp]: "valid_ty_uexpr t \<Longrightarrow> valid_ty_subst sub \<Longrightarrow> valid_ty_uexpr (subst sub t)"
   by (induction t rule: valid_ty_uexpr.induct) 
      (auto simp add: valid_ty_subst_def ran_def split: option.splits)
-
-lemma [simp]: "valid_ty_subst \<Gamma> \<Longrightarrow> valid_ty_subst sub \<Longrightarrow> 
-    valid_ty_subst (map_option (subst sub) \<circ> \<Gamma>)"
-  by (auto simp add: valid_ty_subst_def ran_def)
 
 lemma [elim]: "valid_ty_subst \<Gamma> \<Longrightarrow> \<Gamma> x = Some t \<Longrightarrow> valid_ty_uexpr t"
   by (auto simp add: valid_ty_subst_def ran_def)
@@ -137,13 +156,19 @@ proof (induction ts arbitrary: sub rule: unify'.induct)
   ultimately show ?case by (simp add: valid_ty_uexprs_def split: if_splits)
 next
   case (4 x e ess)
-  from 4 have "e = Var x \<Longrightarrow> valid_ty_uexprs ess \<Longrightarrow> unify' ess = Some xsub \<Longrightarrow> valid_ty_subst xsub" by simp
-  from 4 have "e \<noteq> Var x \<Longrightarrow>
-    x \<notin> vars e \<Longrightarrow> valid_ty_uexprs (list_subst x e ess) \<Longrightarrow> unify' (list_subst x e ess) = Some xsub \<Longrightarrow> valid_ty_subst xsub" by simp
-  from 4 have "valid_ty_uexprs ((Var x, e) # ess)" by simp
-  from 4 have "unify' ((Var x, e) # ess) = Some sub" by simp
-
-  then show ?case by (auto simp add: valid_ty_uexprs_def split: if_splits)
+  thus ?case
+  proof (cases "e = Var x")
+    case False note F = False
+    with 4 show ?thesis 
+    proof (cases "x \<in> vars e")
+      case False
+      with 4 F obtain sub' where S: "unify' (list_subst x e ess) = Some sub' \<and> 
+        sub = extend_subst x e sub'" by auto
+      from 4 have "valid_ty_uexpr e \<and> valid_ty_uexprs ess" by (simp add: valid_ty_uexprs_def)
+      hence "valid_ty_uexprs (list_subst x e ess)" by simp
+      with 4 F False S show ?thesis by (simp add: valid_ty_uexprs_def)
+    qed simp_all
+  qed (simp_all add: valid_ty_uexprs_def)
 qed (auto simp add: valid_ty_uexprs_def)
 
 lemma [elim]: "valid_ty_uexpr t\<^sub>1 \<Longrightarrow> valid_ty_uexpr t\<^sub>2 \<Longrightarrow> unify t\<^sub>1 t\<^sub>2 = Some sub \<Longrightarrow> 
@@ -182,23 +207,17 @@ proof (induction e arbitrary: \<Gamma> vs e' t vs' uni)
   with NLam have "valid_ty_uexpr (Ctor ''Arrow'' [Var ?v, tt]) \<and> 
     valid_ty_hexpr (HLam x (Var ?v) ee')" by simp
   with T show ?case by blast
-next
-  case (NApp e1 e2)
-  from NApp(4) obtain e\<^sub>1' t\<^sub>1 vvs' uni\<^sub>1 e\<^sub>2' t\<^sub>3 uni\<^sub>2 where T: "e' = HApp e\<^sub>1' e\<^sub>2' \<and> 
-    typecheck' \<Gamma> vs e1 = Some (e\<^sub>1', Ctor ''Arrow'' [t\<^sub>1, t], vvs', uni\<^sub>1) \<and> 
-      typecheck' \<Gamma> vvs' e2 = Some (e\<^sub>2', t\<^sub>3, vs', uni\<^sub>2) \<and>
-        uni = (t\<^sub>1, t\<^sub>3) # uni\<^sub>1 @ uni\<^sub>2" 
-          by (auto split: option.splits uexpr.splits list.splits if_splits)
-  moreover with NApp have "valid_ty_uexpr (Ctor ''Arrow'' [t\<^sub>1, t]) \<and> valid_ty_hexpr e\<^sub>1'" by blast
-  moreover with NApp T have "valid_ty_uexpr t\<^sub>3 \<and> valid_ty_hexpr e\<^sub>2'" by blast
-  ultimately show ?case by simp
-qed (auto split: option.splits)
+qed (auto simp add: Let_def split: option.splits)
 
-lemma [elim]: "valid_ty_subst \<Gamma> \<Longrightarrow> typecheck' \<Gamma> vs e = Some (e', t, vs', uni) \<Longrightarrow> 
-    valid_ty_uexpr t"
+lemma [elim]: "valid_ty_subst \<Gamma> \<Longrightarrow> typecheck' \<Gamma> vs e = Some (e', t, vs', uni) \<Longrightarrow> valid_ty_uexpr t"
   by simp
 
-lemma [simp]: "typecheck' \<Gamma> vs e = Some (e', t, vs', uni) \<Longrightarrow> unify' uni = Some sub \<Longrightarrow> 
+lemma [elim]: "valid_ty_subst \<Gamma> \<Longrightarrow> typecheck' \<Gamma> vs e = Some (e', t, vs', uni) \<Longrightarrow> 
+    valid_ty_hexpr e'"
+  by simp
+
+lemma typecheck_succeeds [simp]: "typecheck' \<Gamma> vs e = Some (e', t, vs', uni) \<Longrightarrow> 
+  unify' uni = Some sub \<Longrightarrow> 
     map_option (typeify \<circ> subst sub) \<circ> \<Gamma> \<turnstile>\<^sub>n solidify (hsubst sub e') : typeify (subst sub t)"
 proof (induction e arbitrary: \<Gamma> vs e' t vs' uni sub)
   case (NVar x)
@@ -239,82 +258,62 @@ next
   qed
 next
   case (NApp e\<^sub>1 e\<^sub>2)
-  then obtain e\<^sub>1' t\<^sub>1 xvs' uni\<^sub>1 e\<^sub>2' t\<^sub>3 uni\<^sub>2 where T: "e' = HApp e\<^sub>1' e\<^sub>2' \<and> uni = (t\<^sub>1, t\<^sub>3) # uni\<^sub>1 @ uni\<^sub>2 \<and>
-    typecheck' \<Gamma> vs e\<^sub>1 = Some (e\<^sub>1', Ctor ''Arrow'' [t\<^sub>1, t], xvs', uni\<^sub>1) \<and>
-      typecheck' \<Gamma> xvs' e\<^sub>2 = Some (e\<^sub>2', t\<^sub>3, vs', uni\<^sub>2)" 
-        by (auto split: option.splits if_splits uexpr.splits list.splits)
+  let ?v = "fresh vs"
+  from NApp obtain e\<^sub>1' t\<^sub>1 vs'' uni\<^sub>1 e\<^sub>2' t\<^sub>2 uni\<^sub>2 where E: "e' = HApp e\<^sub>1' e\<^sub>2' \<and> t = Var ?v \<and>
+    typecheck' \<Gamma> (insert ?v vs) e\<^sub>1 = Some (e\<^sub>1', t\<^sub>1, vs'', uni\<^sub>1) \<and>
+      typecheck' \<Gamma> vs'' e\<^sub>2 = Some (e\<^sub>2', t\<^sub>2, vs', uni\<^sub>2) \<and> 
+        uni = (t\<^sub>1, Ctor ''arrow'' [t\<^sub>2, Var ?v]) # uni\<^sub>1 @ uni\<^sub>2" 
+    by (auto simp add: Let_def split: option.splits)
 
 
-  from NApp T have "unify' uni\<^sub>1 = Some sub\<^sub>1 \<Longrightarrow> 
-    map_option (typeify \<circ> subst sub\<^sub>1) \<circ> \<Gamma> \<turnstile>\<^sub>n solidify (hsubst sub\<^sub>1 e\<^sub>1') : typeify (subst sub\<^sub>1 (Ctor ''Arrow'' [t\<^sub>1, t]))" 
-      by blast
-  from NApp T have "unify' uni\<^sub>2 = Some sub\<^sub>2 \<Longrightarrow> 
-    map_option (typeify \<circ> subst sub\<^sub>2) \<circ> \<Gamma> \<turnstile>\<^sub>n solidify (hsubst sub\<^sub>2 e\<^sub>2') : typeify (subst sub\<^sub>2 t\<^sub>3)" by blast
-
+  from NApp E have "unify' uni\<^sub>1 = Some sub\<^sub>1 \<Longrightarrow> 
+    map_option (typeify \<circ> subst sub\<^sub>1) \<circ> \<Gamma> \<turnstile>\<^sub>n solidify (hsubst sub\<^sub>1 e\<^sub>1') : typeify (subst sub\<^sub>1 t\<^sub>1)" by blast
+  from NApp E have "unify' uni\<^sub>2 = Some sub\<^sub>2 \<Longrightarrow> 
+    map_option (typeify \<circ> subst sub\<^sub>2) \<circ> \<Gamma> \<turnstile>\<^sub>n solidify (hsubst sub\<^sub>2 e\<^sub>2') : typeify (subst sub\<^sub>2 t\<^sub>2)" by blast
 
   from NApp have "unify' uni = Some sub" by simp
 
 
 
+  have X: "map_option (typeify \<circ> subst sub) \<circ> \<Gamma> \<turnstile>\<^sub>n solidify (hsubst sub e\<^sub>1') : 
+    Arrow (typeify (subst sub t\<^sub>1)) (typeify (subst sub t))" by simp
 
-  have X: "map_option (typeify \<circ> subst sub) \<circ> \<Gamma> \<turnstile>\<^sub>n solidify (hsubst sub e\<^sub>1') : Arrow xt\<^sub>1 (typeify (subst sub t))" by simp
 
 
-  have "map_option (typeify \<circ> subst sub) \<circ> \<Gamma> \<turnstile>\<^sub>n solidify (hsubst sub e\<^sub>2') : xt\<^sub>1" by simp
+
+  have "map_option (typeify \<circ> subst sub) \<circ> \<Gamma> \<turnstile>\<^sub>n solidify (hsubst sub e\<^sub>2') : typeify (subst sub t\<^sub>1)" 
+    by simp
   with X have "map_option (typeify \<circ> subst sub) \<circ> \<Gamma> \<turnstile>\<^sub>n solidify (hsubst sub (HApp e\<^sub>1' e\<^sub>2')) : 
     typeify (subst sub t)" by simp
-  with T show ?case by blast
+  with E show ?case by blast
 qed
 
 lemma [simp]: "typecheck e = Some (e\<^sub>t, t) \<Longrightarrow> Map.empty \<turnstile>\<^sub>n e\<^sub>t : t"
 proof -
   assume "typecheck e = Some (e\<^sub>t, t)"
-  then obtain e' tt vs \<Gamma> uni sub where T: "typecheck' Map.empty {} e = Some (e', tt, vs, \<Gamma>, uni) \<and>
+  then obtain e' tt vs uni sub where "typecheck' Map.empty {} e = Some (e', tt, vs, uni) \<and>
     unify' uni = Some sub \<and> e\<^sub>t = solidify (hsubst sub e') \<and> t = typeify (subst sub tt)" 
       by (auto split: option.splits)
-
-
-
-  have "Map.empty \<turnstile>\<^sub>n solidify (hsubst sub e') : typeify (subst sub tt)" by simp
-  with T show "Map.empty \<turnstile>\<^sub>n e\<^sub>t : t" by simp
+  moreover hence "map_option (typeify \<circ> subst sub) \<circ> Map.empty \<turnstile>\<^sub>n solidify (hsubst sub e') : 
+    typeify (subst sub tt)" by (metis typecheck_succeeds)
+  ultimately show "Map.empty \<turnstile>\<^sub>n e\<^sub>t : t" by simp
 qed
 
-lemma erase_solidify [simp]: "valid_ty_subst \<Gamma> \<Longrightarrow> typecheck' \<Gamma> vs e = Some (e', t, vs', \<Gamma>') \<Longrightarrow> 
-  e = erase (solidify e')"
-proof (induction e arbitrary: \<Gamma> vs e' t vs' \<Gamma>')
-  case (NLam x e)
-  let ?v = "fresh vs"
-  from NLam(3) obtain ee' tt g\<Gamma>' t' where T: "g\<Gamma>' x = Some t' \<and> e' = HLam x t' ee' \<and> 
-    t = Ctor ''Arrow'' [t', tt] \<and> \<Gamma>' = g\<Gamma>'(x := \<Gamma> x) \<and> 
-      typecheck' (\<Gamma>(x \<mapsto> Var ?v)) (insert ?v vs) e = Some (ee', tt, vs', g\<Gamma>')" 
-    by (auto simp add: Let_def split: option.splits)
-  from NLam have "valid_ty_subst (\<Gamma>(x \<mapsto> Var ?v))" by simp
-  with NLam(1) T have "e = erase (solidify ee')" by blast
-  with T show ?case by simp
-next
-  case (NApp e1 e2)
-  from NApp(4) obtain e\<^sub>1' t\<^sub>1 t\<^sub>2 vvs' g\<Gamma>' e\<^sub>2' t\<^sub>3 g\<Gamma>'' sub where T: "unify t\<^sub>1 t\<^sub>2 = Some sub \<and> 
-    t = subst sub t\<^sub>2 \<and> e' = HApp (hsubst sub e\<^sub>1') (hsubst sub e\<^sub>2') \<and> 
-      \<Gamma>' = map_option (subst sub) \<circ> g\<Gamma>'' \<and> 
-        typecheck' \<Gamma> vs e1 = Some (e\<^sub>1', Ctor ''Arrow'' [t\<^sub>1, t\<^sub>2], vvs', g\<Gamma>') \<and>
-          typecheck' g\<Gamma>' vvs' e2 = Some (e\<^sub>2', t\<^sub>3, vs', g\<Gamma>'')" 
-    by (auto split: option.splits prod.splits uexpr.splits list.splits if_splits)
-  moreover with NApp(3) have X: "valid_ty_subst g\<Gamma>' \<and> valid_ty_uexpr (Ctor ''Arrow'' [t\<^sub>1, t\<^sub>2]) \<and> 
-    valid_ty_hexpr e\<^sub>1'" by fastforce
-  moreover with T have "valid_ty_subst g\<Gamma>'' \<and> valid_ty_uexpr t\<^sub>3 \<and> valid_ty_hexpr e\<^sub>2'" by fastforce
-  moreover from NApp T have "e1 = erase (solidify e\<^sub>1')" by blast
-  moreover from NApp T X have "e2 = erase (solidify e\<^sub>2')" by blast
-  ultimately show ?case by simp
-qed (auto simp add: Let_def split: option.splits)
+lemma erase_solidify [simp]: "typecheck' \<Gamma> vs e = Some (e', t, vs', uni) \<Longrightarrow> 
+    e = erase (solidify e')"
+  by (induction e arbitrary: \<Gamma> vs e' t vs' uni) 
+     (auto simp add: Let_def split: option.splits)
 
 lemma [simp]: "typecheck e = Some (e\<^sub>t, t) \<Longrightarrow> e = erase e\<^sub>t"
 proof -
   assume "typecheck e = Some (e\<^sub>t, t)"
-  then obtain e' tt vs \<Gamma> where T: "typecheck' Map.empty {} e = Some (e', tt, vs, \<Gamma>) \<and> 
-    e\<^sub>t = solidify e' \<and> t = typeify tt" by (auto split: option.splits)
-  moreover have "valid_ty_subst Map.empty" by simp
-  ultimately have "e = erase (solidify e')" by (metis erase_solidify)
-  with T show ?thesis by simp
+  then obtain e' tt vs uni sub where T: "typecheck' Map.empty {} e = Some (e', tt, vs, uni) \<and> 
+    unify' uni = Some sub \<and> e\<^sub>t = solidify (hsubst sub e') \<and> t = typeify (subst sub tt)" 
+      by (auto split: option.splits)
+  hence X: "e = erase (solidify e')" by (metis erase_solidify)
+  have "valid_ty_subst Map.empty" by simp
+  with T have "valid_ty_hexpr e'" by fastforce
+  with T X show ?thesis by simp
 qed
 
 lemma [dest]: "erase e\<^sub>t = NVar x \<Longrightarrow> e\<^sub>t = TVar x"
@@ -333,39 +332,35 @@ proof (induction e arbitrary: \<Gamma> vs e\<^sub>t t)
 next
   case (NLam x e)
   let ?v = "fresh vs"
-  show ?case
-  proof (cases "typecheck' (\<Gamma>(x \<mapsto> Var ?v)) (insert ?v vs) e")
-    case None
-
-    from NLam obtain t\<^sub>1 e\<^sub>t' where E: "e\<^sub>t = TLam x t\<^sub>1 e\<^sub>t' \<and> e = erase e\<^sub>t'" by blast
-    from NLam E obtain t\<^sub>2 where "((map_option typeify \<circ> \<Gamma>)(x \<mapsto> t\<^sub>1) \<turnstile>\<^sub>n e\<^sub>t' : t\<^sub>2) \<and> t = Arrow t\<^sub>1 t\<^sub>2" 
-      by blast
-
-
-
-    have "(map_option typeify \<circ> \<Gamma>)(x \<mapsto> TyVar ?v) \<turnstile>\<^sub>n e\<^sub>t' : xt" by simp
-    hence "map_option typeify \<circ> (\<Gamma>(x \<mapsto> Var ?v)) \<turnstile>\<^sub>n e\<^sub>t' : xt" by simp
-    with NLam E None show ?thesis by blast
-  next
-    case (Some a)
-    with NLam obtain e' t' vs' \<Gamma>' where G: "\<Gamma>' x = None \<and> 
-      typecheck' (\<Gamma>(x \<mapsto> Var ?v)) (insert ?v vs) e = Some (e', t', vs', \<Gamma>')" 
-        by (auto simp add: Let_def split: option.splits prod.splits)
-    hence "dom \<Gamma>' = dom (\<Gamma>(x \<mapsto> Var ?v))" by force
-    with G show ?thesis by auto
-  qed
+  from NLam have T: "typecheck' (\<Gamma>(x \<mapsto> Var ?v)) (insert ?v vs) e = None" 
+    by (auto simp add: Let_def split: option.splits)
+  from NLam obtain t\<^sub>1 e\<^sub>t' where E: "e\<^sub>t = TLam x t\<^sub>1 e\<^sub>t' \<and> e = erase e\<^sub>t'" by auto
+  with NLam obtain t\<^sub>2 where "t = Arrow t\<^sub>1 t\<^sub>2 \<and> (map_option typeify \<circ> \<Gamma>)(x \<mapsto> t\<^sub>1) \<turnstile>\<^sub>n e\<^sub>t' : t\<^sub>2" by blast
+  hence "map_option typeify \<circ> (\<Gamma>(x \<mapsto> Var ?v)) \<turnstile>\<^sub>n e\<^sub>t' : t\<^sub>2" by simp
+  with NLam T E show ?case by blast
 next
   case (NApp e1 e2)
   thus ?case by simp
 qed simp_all
 
 lemma typecheck_fails [simp]: "typecheck e = None \<Longrightarrow> \<nexists>e\<^sub>t t. (Map.empty \<turnstile>\<^sub>n e\<^sub>t : t) \<and> e = erase e\<^sub>t"
-proof 
-  assume "typecheck e = None"
-  hence X: "typecheck' Map.empty {} e = None" by (simp split: option.splits prod.splits)
+proof (rule, cases "typecheck' Map.empty {} e")
+  case None
   assume "\<exists>e\<^sub>t t. (Map.empty \<turnstile>\<^sub>n e\<^sub>t : t) \<and> e = erase e\<^sub>t"
-  then obtain e\<^sub>t t where "(map_option typeify \<circ> Map.empty \<turnstile>\<^sub>n e\<^sub>t : t) \<and> e = erase e\<^sub>t" by fastforce
-  with X show "False" by (metis typecheck_fails')
+  then obtain e\<^sub>t tt where "(map_option typeify \<circ> Map.empty \<turnstile>\<^sub>n e\<^sub>t : tt) \<and> e = erase e\<^sub>t" by fastforce
+  with None show "False" by (metis typecheck_fails')
+next
+  case (Some out)
+  moreover assume "typecheck e = None"
+  ultimately obtain e' t vs uni where X: "typecheck' Map.empty {} e = Some (e', t, vs, uni) \<and> 
+    unify' uni = None" by (auto split: option.splits prod.splits)
+
+
+  assume "\<exists>e\<^sub>t t. (Map.empty \<turnstile>\<^sub>n e\<^sub>t : t) \<and> e = erase e\<^sub>t"
+  then obtain e\<^sub>t tt where "(map_option typeify \<circ> Map.empty \<turnstile>\<^sub>n e\<^sub>t : tt) \<and> e = erase e\<^sub>t" by fastforce
+
+
+  with Some X show "False" by simp
 qed
 
 lemma [simp]: "valn (erase e) = valt e"
@@ -395,47 +390,49 @@ lemma [simp]: "tsubstt sub (substt x v e) = substt x (tsubstt sub v) (tsubstt su
 lemma [simp]: "e \<Down>\<^sub>t v \<Longrightarrow> tsubstt sub e \<Down>\<^sub>t tsubstt sub v"
   by (induction e v rule: evalt.induct) simp_all
 
-lemma correctness' [simp]: "e \<Down> v \<Longrightarrow> typecheck' \<Gamma> vs e = Some (e\<^sub>t, t1, vs', \<Gamma>') \<Longrightarrow> 
-  typecheck' \<Gamma> vs v = Some (v\<^sub>t, t2, vs'', \<Gamma>'') \<Longrightarrow> valid_ty_subst \<Gamma> \<Longrightarrow> typeify t1 = typeify t2 \<Longrightarrow> 
-    solidify e\<^sub>t \<Down>\<^sub>t solidify v\<^sub>t"
-proof (induction e v arbitrary: \<Gamma> vs e\<^sub>t t1 vs' \<Gamma>' v\<^sub>t t2 vs'' \<Gamma>'' rule: evaln.induct)
+lemma correctness' [simp]: "e \<Down> v \<Longrightarrow> typecheck' \<Gamma> vs e = Some (e\<^sub>t, t1, vs1, uni1) \<Longrightarrow> 
+  typecheck' \<Gamma> vs v = Some (v\<^sub>t, t2, vs2, uni2) \<Longrightarrow> valid_ty_subst \<Gamma> \<Longrightarrow> unify' uni1 = Some sub1 \<Longrightarrow> 
+    unify' uni2 = Some sub2 \<Longrightarrow> typeify (subst sub1 t1) = typeify (subst sub2 t2) \<Longrightarrow> 
+      solidify (hsubst sub1 e\<^sub>t) \<Down>\<^sub>t solidify (hsubst sub2 v\<^sub>t)"
+proof (induction e v arbitrary: vs e\<^sub>t t1 vs1 uni1 v\<^sub>t t2 vs2 uni2 sub1 sub2 rule: evaln.induct)
   case (evn_app e\<^sub>1 x e\<^sub>1' e\<^sub>2 v\<^sub>2 v)
-  from evn_app(7) obtain e\<^sub>1'' t\<^sub>1 t\<^sub>2 vs\<^sub>1' \<Gamma>\<^sub>1' e\<^sub>2' t\<^sub>3 \<Gamma>\<^sub>2' sub where T: "t1 = subst sub t\<^sub>2 \<and> 
-    e\<^sub>t = HApp (hsubst sub e\<^sub>1'') (hsubst sub e\<^sub>2') \<and> \<Gamma>' = map_option (subst sub) \<circ> \<Gamma>\<^sub>2' \<and>
-      typecheck' \<Gamma> vs e\<^sub>1 = Some (e\<^sub>1'', Ctor ''Arrow'' [t\<^sub>1, t\<^sub>2], vs\<^sub>1', \<Gamma>\<^sub>1') \<and>
-        typecheck' \<Gamma>\<^sub>1' vs\<^sub>1' e\<^sub>2 = Some (e\<^sub>2', t\<^sub>3, vs', \<Gamma>\<^sub>2') \<and> unify t\<^sub>1 t\<^sub>2 = Some sub" 
-    by (auto split: option.splits if_splits uexpr.splits list.splits)
-  with evn_app(9) have X: "valid_ty_subst \<Gamma>\<^sub>1' \<and> valid_ty_uexpr (Ctor ''Arrow'' [t\<^sub>1, t\<^sub>2]) \<and> 
-    valid_ty_hexpr e\<^sub>1''" by fastforce
-  with T have Y: "valid_ty_subst \<Gamma>\<^sub>2' \<and> valid_ty_uexpr t\<^sub>3 \<and> valid_ty_hexpr e\<^sub>2'" by fastforce
-
-
-  from evn_app T have "typecheck' \<Gamma> vs (NLam x e\<^sub>1') = Some (xv\<^sub>t, xt2, xvs'', x\<Gamma>'') \<Longrightarrow> 
-    Arrow (typeify t\<^sub>1) (typeify t\<^sub>2) = typeify xt2 \<Longrightarrow> solidify e\<^sub>1'' \<Down>\<^sub>t solidify xv\<^sub>t" by auto
-
-  from evn_app T have "typecheck' \<Gamma>\<^sub>1' vs\<^sub>1' v\<^sub>2 = Some (xv\<^sub>t, xt2, xvs'', x\<Gamma>'') \<Longrightarrow> 
-    typeify t\<^sub>3 = typeify xt2 \<Longrightarrow> valid_ty_subst \<Gamma>\<^sub>1' \<Longrightarrow> solidify e\<^sub>2' \<Down>\<^sub>t solidify xv\<^sub>t" by blast
+  let ?v = "fresh vs"
+  from evn_app obtain e\<^sub>t\<^sub>1 t\<^sub>1 vs'' uni\<^sub>1 e\<^sub>t\<^sub>2 t\<^sub>2 uni\<^sub>2 where E: "e\<^sub>t = HApp e\<^sub>t\<^sub>1 e\<^sub>t\<^sub>2 \<and> t1 = Var ?v \<and>
+    typecheck' \<Gamma> (insert ?v vs) e\<^sub>1 = Some (e\<^sub>t\<^sub>1, t\<^sub>1, vs'', uni\<^sub>1) \<and>
+      typecheck' \<Gamma> vs'' e\<^sub>2 = Some (e\<^sub>t\<^sub>2, t\<^sub>2, vs1, uni\<^sub>2) \<and> 
+        uni1 = (t\<^sub>1, Ctor ''arrow'' [t\<^sub>2, Var ?v]) # uni\<^sub>1 @ uni\<^sub>2" 
+    by (auto simp add: Let_def split: option.splits)
 
   from evn_app have "e\<^sub>1 \<Down> NLam x e\<^sub>1'" by simp
   from evn_app have "e\<^sub>2 \<Down> v\<^sub>2" by simp
   from evn_app have "substn x v\<^sub>2 e\<^sub>1' \<Down> v" by simp
+  from evn_app E have "typecheck' \<Gamma> (insert ?v vs) (NLam x e\<^sub>1') = Some (xv\<^sub>t, xt20, xvs20, xuni20) \<Longrightarrow>
+    unify' uni\<^sub>1 = Some xsub1 \<Longrightarrow>
+    unify' xuni20 = Some xsub2 \<Longrightarrow>
+    typeify (subst xsub1 t\<^sub>1) = typeify (subst xsub2 xt20) \<Longrightarrow> solidify (hsubst xsub1 e\<^sub>t\<^sub>1) \<Down>\<^sub>t solidify (hsubst xsub2 xv\<^sub>t)" by blast
+  from evn_app have "typecheck' \<Gamma> xvs e\<^sub>2 = Some (xe\<^sub>t, xt10, xvs10, xuni10) \<Longrightarrow>
+    typecheck' \<Gamma> xvs v\<^sub>2 = Some (xv\<^sub>t, xt20, xvs20, xuni20) \<Longrightarrow>
+    unify' xuni10 = Some xsub1 \<Longrightarrow>
+    unify' xuni20 = Some xsub2 \<Longrightarrow>
+    typeify (subst xsub1 xt10) = typeify (subst xsub2 xt20) \<Longrightarrow> solidify (hsubst xsub1 xe\<^sub>t) \<Down>\<^sub>t solidify (hsubst xsub2 xv\<^sub>t)" by simp
+  from evn_app have "typecheck' \<Gamma> xvs (substn x v\<^sub>2 e\<^sub>1') = Some (xe\<^sub>t, xt10, xvs10, xuni10) \<Longrightarrow>
+    typecheck' \<Gamma> xvs v = Some (xv\<^sub>t, xt20, xvs20, xuni20) \<Longrightarrow>
+    unify' xuni10 = Some xsub1 \<Longrightarrow>
+    unify' xuni20 = Some xsub2 \<Longrightarrow>
+    typeify (subst xsub1 xt10) = typeify (subst xsub2 xt20) \<Longrightarrow> solidify (hsubst xsub1 xe\<^sub>t) \<Down>\<^sub>t solidify (hsubst xsub2 xv\<^sub>t)" by simp
+  from evn_app have "typecheck' \<Gamma> vs v = Some (v\<^sub>t, t2, vs2, uni2)" by simp
+  from evn_app have "valid_ty_subst \<Gamma>" by simp
+  from evn_app have "unify' uni1 = Some sub1" by simp
+  from evn_app have "unify' uni2 = Some sub2" by simp
+  from evn_app have "typeify (subst sub1 t1) = typeify (subst sub2 t2)" by simp
 
 
-
-
-  from evn_app have "typecheck' x\<Gamma> xvs (substn x v\<^sub>2 e\<^sub>1') = Some (xe\<^sub>t, xt1, xvs', x\<Gamma>') \<Longrightarrow>
-    typecheck' x\<Gamma> xvs v = Some (xv\<^sub>t, xt2, xvs'', x\<Gamma>'') \<Longrightarrow> valid_ty_subst x\<Gamma> \<Longrightarrow> typeify xt1 = typeify xt2 \<Longrightarrow> 
-      solidify xe\<^sub>t \<Down>\<^sub>t solidify xv\<^sub>t" by simp
-  from evn_app have "typecheck' \<Gamma> vs v = Some (v\<^sub>t, t2, vs'', \<Gamma>'')" by simp
-  from evn_app have "typeify t1 = typeify t2" by simp
-
-
-  have "tsubstt sub (TApp (solidify e\<^sub>1'') (solidify e\<^sub>2')) \<Down>\<^sub>t solidify v\<^sub>t" by simp
-  with T X Y show ?case by simp
-qed (auto simp add: Let_def split: option.splits)
+  have "solidify (hsubst sub1 e\<^sub>t) \<Down>\<^sub>t solidify (hsubst sub2 v\<^sub>t)" by simp
+  thus ?case by simp
+qed (auto simp add: Let_def split: option.splits prod.splits)
 
 theorem correctness: "e \<Down> v \<Longrightarrow> typecheck e = Some (e\<^sub>t, t) \<Longrightarrow> typecheck v = Some (v\<^sub>t, t) \<Longrightarrow> 
     e\<^sub>t \<Down>\<^sub>t v\<^sub>t"
-  by (auto split: option.splits)
+  by (auto split: option.splits prod.splits)
 
 end
